feat(davi): Ex5: improve Valid and implement mem

davi_solutions/Ex5.dfy
@@ -8,18 +8,68 @@ module Ex5 {
     var tbl : array<bool>  
     var list : Ex3.Node?
 
-    ghost function Valid() : bool 
-    {
+    ghost var footprint: set<Ex3.Node>
+    ghost var content: set<nat>
+    ghost var tblSeq: seq<bool>
 
+    // If something is in the set than that entry is true in tbl
+    ghost function Valid() : bool 
+      reads this, this.footprint, this.list, this.tbl
+    {
+      if (this.list == null)
+        then
+          |this.tblSeq| == this.tbl.Length
+          && 
+          this.footprint == {}
+          &&
+          this.content == {}
+          &&
+          (forall k :: 0 <= k < |this.tblSeq| ==> this.tblSeq[k] == false)
+          &&
+          forall k :: 0 <= k < |this.tblSeq| ==> this.tblSeq[k] == this.tbl[k]
+        else 
+          |this.tblSeq| == this.tbl.Length
+          && 
+          this.footprint == this.list.footprint
+          && 
+          this.content == this.list.content
+          && 
+          this.list.Valid()
+          && 
+          (forall k :: 0 <= k < |this.tblSeq| ==> this.tblSeq[k] == this.tbl[k])
+          && 
+          forall k :: 0 <= k < |this.tblSeq| ==> this.tblSeq[k] == true <==> k in this.content
     }
       
     constructor (size : nat) 
+      ensures this.Valid() && this.content == {} && this.footprint == {}
+      ensures |this.tblSeq| == size + 1
+      ensures forall k :: 0 <= k < |this.tblSeq| ==> this.tblSeq[k] == false
     {
+      var aux := new bool[size + 1];
+      var i := 0;
+      while (i < aux.Length)
+        invariant 0 <= i <= aux.Length
+        invariant forall k :: 0 <= k < i ==> aux[k] == false
+      {
+        aux[i] := false;
+        i := i + 1;
+      }
+      this.list := null;
+      this.tbl := aux;
+      this.tblSeq := aux[..];
+      this.footprint := {};
+      this.content := {};
     }
 
-
     method mem (v : nat) returns (b : bool)
+      requires this.Valid()
+      ensures v < |this.tblSeq| ==> b == (v in this.content)
     {
+      b := false;
+      if (v < tbl.Length){
+        b := tbl[v];
+      }
     }
     
     method add (v : nat) 
